implemented finite oraclestate

Structures/FixedMap.v
@@ -3,6 +3,7 @@ Require Import ssreflect ssrbool ssrnat eqtype fintype choice ssrfun seq path.
 
 From Probchain
 Require Import FixedList.
+Set Implicit Arguments.
 
 
 
@@ -18,31 +19,30 @@ Section fixmap.
 
     Definition fixmap_empty n : fixmap n :=
         FixMap
-            n
             (fixlist_empty K n)
             (fixlist_empty V n).
             
     Definition fixmap_find (k : K) (n : nat) (map : fixmap n) : option V :=
-        match (fixlist_index_of k (fixmap_key n map)) with
+        match (fixlist_index_of k (fixmap_key  map)) with
             | None => None
-            | Some index => fixlist_get_nth (fixmap_value n map) index
+            | Some index => fixlist_get_nth (fixmap_value  map) index
         end.
 
 
     Definition fixmap_put (k : K) (v : V) (n : nat) (map : fixmap n) : fixmap n :=
-        match (fixlist_index_of k (fixmap_key n map)) with
-            | None => let: keys := (fixlist_insert (fixmap_key n map) k) in
-                        match (fixlist_index_of k (fixmap_key n map)) with
+        match (fixlist_index_of k (fixmap_key  map)) with
+            | None => let: keys := (fixlist_insert (fixmap_key  map) k) in
+                        match (fixlist_index_of k (fixmap_key  map)) with
                             | None => map (* keys list is full, ignore put *)
-                            | Some index => let: values := (fixlist_set_nth (fixmap_value n map) v index) in
-                                            FixMap n keys values
+                            | Some index => let: values := (fixlist_set_nth (fixmap_value  map) v index) in
+                                            FixMap  keys values
                         end
-            | Some index => let: keys := (fixlist_insert (fixmap_key n map) k) in
-                            let: values := (fixlist_set_nth (fixmap_value n map) v index) in
-                                            FixMap n keys values
+            | Some index => let: keys := (fixlist_insert (fixmap_key  map) k) in
+                            let: values := (fixlist_set_nth (fixmap_value  map) v index) in
+                                            FixMap  keys values
             end.
 
-    Lemma fixmap_ident (n : nat) (map : fixmap n) : n > 0 -> forall k v, fixmap_find k n (fixmap_put k v n map) = Some v.
+    Lemma fixmap_ident (n : nat) (map : fixmap n) : n > 0 -> forall k v, fixmap_find k  (fixmap_put k v  map) = Some v.
     Proof.
         move=> H.
         (* TODO(Kiran): Complete this proof. *)
